Common/Common.v
@@ -10,6 +10,7 @@ From stdpp Require Export pretty.
 From stdpp Require Export vector.
 From stdpp Require Export finite.
 From stdpp Require Export relations.
+From stdpp Require Export propset.
 Require Export Ensembles.
 
 Require Export CBase.
@@ -21,52 +22,14 @@ Require Export CSets.
 Require Export CMaps.
 Require Export CInduction.
 
-(*** Utility functions ***)
+(** * Utility functions ***)
 
 (** Update a function at a specific value *)
 Definition fun_add {A B} {_: EqDecision A} (k : A) (v : B) (f : A -> B) :=
   fun x : A => if k =? x then v else f x.
 
 
-(*** Ensembles ***)
-(* I really don't understand why this is not in stdpp *)
-(* stdpp use propset instead of Ensemble, maybe that would be better *)
-
-Global Instance Ensemble_elem_of {A} : ElemOf A (Ensemble A) := fun x P => P x.
-
-Global Instance Ensemble_empty {A} : Empty (Ensemble A) := fun a => False.
-
-Global Instance Ensemble_singleton {A} :
-  Singleton A (Ensemble A) := fun x y => x = y.
-
-Global Instance Ensemble_union {A} :
-  Union (Ensemble A) := fun P Q x => P x \/ Q x.
-Global Instance Ensemble_intersection {A} :
-  Intersection (Ensemble A) := fun P Q x => P x /\ Q x.
-
-Global Instance Ensemble_difference {A} :
-  Difference (Ensemble A) := fun P Q x => P x /\ ¬(Q x).
-
-
-Global Instance Ensemble_mbind : MBind Ensemble := λ A B f E b,
-    ∃'a ∈ E, b ∈ f a.
-
-Global Instance Ensemble_omap : OMap Ensemble := λ A B f E b,
-    ∃'a ∈ E, f a = Some b.
-
-
-Definition Ensemble_from_set {A C} `{ElemOf A C} (c : C) : Ensemble A := fun a => a ∈ c.
-
-Global Instance Ensemble_SemiSet A : SemiSet A (Ensemble A).
-Proof. sauto l:on. Qed.
-
-Global Instance Ensemble_Set A : Set_ A (Ensemble A).
-Proof. sauto l:on. Qed.
-
-
 (** * Vectors ***)
-
-
 
 Section VAlter.
   Context {A : Type}.
@@ -119,9 +82,40 @@ Create HintDb vec discriminated.
 #[global] Hint Rewrite @valter_eq using done : vec.
 #[global] Hint Rewrite @vec_to_list_length : vec.
 
+Section VecLookup.
+  Context {T : Type}.
+  Context {n : nat}.
+
+  Global Instance vec_lookup_nat : Lookup nat T (vec T n) :=
+    fun m v =>
+      match decide (m < n) with
+      | left H => Some (v !!! Fin.of_nat_lt H)
+      | right _ => None
+      end.
+
+  Lemma vec_to_list_lookup (v : vec T n) m : vec_to_list v !! m = v !! m.
+  Proof using.
+    unfold lookup at 2.
+    unfold vec_lookup_nat.
+    case_decide.
+    - apply vlookup_lookup'.
+      naive_solver.
+    - apply lookup_ge_None.
+      rewrite vec_to_list_length.
+      lia.
+  Qed.
+
+  Global Instance vec_lookup_nat_unfold m (v : vec T n) r:
+    LookupUnfold m v r →
+    LookupUnfold m (vec_to_list v) r.
+  Proof using. tcclean. apply vec_to_list_lookup. Qed.
+
+  Global Instance vec_lookup_N : Lookup N T (vec T n) :=
+    fun m v => v !! (N.to_nat m).
+End VecLookup.
 
 
-(*** Finite decidable quantifiers ***)
+(** * Finite decidable quantifiers ***)
 
 (* TODO maybe express with a decidable instance instead : There are consequences
    for extraction though
@@ -155,10 +149,7 @@ Proof.
 Qed.
 
 
-(*** Finite number utilities ***)
-
-(* TODO upstream to stdpp *)
-Bind Scope fin_scope with fin.
+(** * Finite number utilities ***)
 
 Global Instance pretty_fin (n : nat) : Pretty (fin n)  :=
   (fun n => pretty (n : nat)).
@@ -166,38 +157,3 @@ Global Hint Mode Pretty ! : typeclass_instances.
 
 Definition fin_to_N {n : nat} : fin n → N := N.of_nat ∘ fin_to_nat.
 Coercion fin_to_N : fin >-> N.
-
-
-
-(*** VectorLookup ***)
-Section VecLookup.
-  Context {T : Type}.
-  Context {n : nat}.
-
-  Global Instance vec_lookup_nat : Lookup nat T (vec T n) :=
-    fun m v =>
-      match decide (m < n) with
-      | left H => Some (v !!! Fin.of_nat_lt H)
-      | right _ => None
-      end.
-
-  Lemma vec_to_list_lookup (v : vec T n) m : vec_to_list v !! m = v !! m.
-  Proof using.
-    unfold lookup at 2.
-    unfold vec_lookup_nat.
-    case_decide.
-    - apply vlookup_lookup'.
-      naive_solver.
-    - apply lookup_ge_None.
-      rewrite vec_to_list_length.
-      lia.
-  Qed.
-
-  Global Instance vec_lookup_nat_unfold m (v : vec T n) r:
-    LookupUnfold m v r →
-    LookupUnfold m (vec_to_list v) r.
-  Proof using. tcclean. apply vec_to_list_lookup. Qed.
-
-  Global Instance vec_lookup_N : Lookup N T (vec T n) :=
-    fun m v => v !! (N.to_nat m).
-End VecLookup.
